Refs are done

my_steps/Pulse.Ch2.fst
@@ -1,6 +1,7 @@
 module Pulse.Ch2
 
 open Pulse.Lib.Pervasives
+open FStar.Mul
 
 // # Mutable References
 
@@ -20,4 +21,226 @@ ensures pts_to r0 'v1 ** pts_to r1 'v0
 ```
 
 // ## Reading a reference
+```pulse
+fn value_of (#a:Type) (r:ref a)
+requires pts_to r 'v
+returns v:a
+ensures pts_to r 'v ** pure (v == 'v)
+{
+  !r;
+}
+```
 
+```pulse
+fn value_of_explicit (#a:Type) (r:ref a) (#w:erased a)
+requires pts_to r w
+returns v:a
+ensures pts_to r w ** pure (v == reveal w)
+{
+  !r;
+}
+```
+
+// ## Erased values are for specification and proof only
+
+// ```pulse
+// fn value_of_explicit_fail (#a:Type) (r:ref a) (#w:erased a)
+// requires pts_to r w
+// returns v:a
+// ensures pts_to r w ** pure (v == reveal w)
+// {
+//     reveal w // error: Expected a Total computation, but got Ghost
+// }
+// ```
+
+// ## Writing through a reference
+
+```pulse
+fn assign (#a:Type) (r:ref a) (v:a)
+requires pts_to r 'v
+ensures pts_to r v
+{
+  r := v;
+}
+```
+
+// ## Dereferencing is explicit
+
+```pulse
+fn add (r:ref int) (n:int)
+requires pts_to r 'v
+ensures pts_to r ('v + n)
+{
+  let v = !r;
+  r := v + n;
+}
+```
+
+```pulse
+fn quadruple (r:ref int)
+requires pts_to r 'v
+ensures pts_to r (4 * 'v)
+{
+  let v1 = !r;
+  add r v1;
+  // show_proof_state;
+  let v2 = !r;
+  add r v2;
+}
+```
+
+// ## Stateful commands are explicitly sequenced
+
+[@expect_failure]
+```pulse
+fn quad_fail (r:ref int)
+requires pts_to r 'v
+ensures pts_to r (4 * 'v)
+{
+  add r (!r);
+  add r (!r);
+}
+```
+// - Expected type "int"; but "!r" has type
+//   "stt int
+//        (pts_to r (reveal (*?u93*) _))
+//        (fun x -> pts_to r x ** pure (reveal (*?u93*) _ == x))"
+
+// ## Fractional Permissions
+
+// open PulseCore.FractionalPermission
+
+```pulse
+fn assign_full_perm (#a:Type) (r:ref a) (v:a)
+requires pts_to r #full_perm 'v
+ensures pts_to r #full_perm v
+{
+  r := v;
+}
+```
+
+```pulse
+fn value_of_perm #a #p (r:ref a)
+requires pts_to r #p 'v
+returns v:a
+ensures pts_to r #p 'v ** pure (v == 'v)
+{
+  !r;
+}
+```
+
+#push-options "--print_implicits"
+[@expect_failure] // If we try to write to a reference without holding full permission on it, Pulse rejects the program, as shown below
+```pulse
+fn assign_perm #a #p (r:ref a) (v:a) (#w: erased a)
+requires pts_to r #p w
+ensures pts_to r #p w
+{
+  r := v;
+}
+```
+#pop-options
+
+```pulse
+fn share_ref #a #p (r:ref a)
+requires pts_to r #p 'v
+ensures pts_to r #(half_perm p) 'v ** pts_to r #(half_perm p) 'v
+{
+  share r;
+}
+```
+
+
+```pulse
+fn gather_ref #a #p (r:ref a)
+requires 
+  pts_to r #(half_perm p) 'v0 **
+  pts_to r #(half_perm p) 'v1
+ensures pts_to r #p 'v0 ** pure ('v0 == 'v1)
+{
+  gather r;
+}
+```
+
+// # Stack references
+
+// let mut creates a new stack ref
+
+```pulse // I copied the incr code from the previous chapter
+fn incr (r:ref int)
+requires pts_to r 'v
+ensures pts_to r ('v + 1)
+{
+    let v = !r;
+    r := v + 1;
+}
+```
+
+```pulse
+fn one()
+requires emp
+returns v:int
+ensures pure (v == 1)
+{
+                 // .          |- emp
+  let mut i = 0; // i: ref int |- pts_to i 0
+  incr i;        // i: ref int |- pts_to i (0 + 1)
+  !i             // .          |- v:int. emp ** pure (v == 1)
+}
+```
+
+// ## Stack references are scoped and implicitly reclaimed
+
+[@expect_failure]
+```pulse
+fn refs_are_scoped ()
+requires emp
+returns s:ref int
+ensures pts_to s 0
+{
+    let mut s = 0;
+    s
+  // - Cannot prove:
+  //     pts_to s 0
+  // - In the context:
+  //     emp
+}
+```
+
+// # Heap references
+
+module Box = Pulse.Lib.Box
+
+```pulse
+fn new_heap_ref (#a: Type) (v: a)
+requires emp
+returns r:Box.box a
+ensures Box.pts_to r v
+{
+  Box.alloc v
+}
+```
+
+```pulse
+fn last_value_off #a (r:Box.box a)
+requires Box.pts_to r 'v
+returns v:a
+ensures pure (v == 'v)
+{
+  open Box;
+  let v = !r;
+  free r;
+  v
+}
+```
+
+```pulse
+fn incr_box (r:Box.box int)
+requires Box.pts_to r 'v
+ensures Box.pts_to r ('v + 1)
+{
+  Box.to_ref_pts_to r;     // Box.pts_to (box_to_ref r) 'v
+  incr (Box.box_to_ref r); // pts_to (box_to_ref r) ('v + 1)
+  Box.to_box_pts_to r      // Box.pts_to r ('v + 1)
+}
+```
